Fix ec specs to match final yul model

src/specs/PointMulIntoDest.ec
@@ -6,48 +6,38 @@ require import Logic.
 require import Memory.
 require import PurePrimops.
 require import Real.
+require import RevertWithMessage.
 require import UInt256.
 require import Utils.
 require import YulPrimops.
 require import Verifier.
 
-import MemoryMap.
-
 module PointMulIntoDest = {
-  proc low(usr_point, usr_s, usr_dest) =
+  proc low(point, s, dest) =
   {
     var _1, _5,  _9, _10;
-    _1 <@ Primops.mload(usr_point);
+    _1 <@ Primops.mload(point);
     Primops.mstore(W256.zero, _1);
-    _5 <@ Primops.mload(usr_point + W256.of_int 32);
+    _5 <@ Primops.mload(point + W256.of_int 32);
     Primops.mstore(W256.of_int 32, _5);
-    Primops.mstore(W256.of_int 64, usr_s);
+    Primops.mstore(W256.of_int 64, s);
     _9 <@ Primops.gas();
-    _10 <@ Primops.staticcall(_9, W256.of_int 7, W256.zero, W256.of_int 96, usr_dest, W256.of_int 64);
+    _10 <@ Primops.staticcall(_9, W256.of_int 7, W256.zero, W256.of_int 96, dest, W256.of_int 64);
     if (bool_of_uint256 (PurePrimops.iszero(_10)))
     {
-      Verifier.usr_revertWithMessage(W256.of_int 30, W256.zero);
+      RevertWithMessage.low(W256.of_int 30, W256.zero);
     }
   }
 }.
 
-lemma usr_pointMulIntoDest_actual_matches_low (x y : uint256) : equiv [
-    Verifier.usr_pointMulIntoDest ~ PointMulIntoDest.low :
-      ={Primops.memory} /\
-      ={arg} /\
-      ={Primops.reverted} /\
-      !Primops.reverted{1}
-      ==>
-        (Primops.reverted{1} <=> Primops.reverted{2}) /\
-        (!Primops.reverted{1}) =>
-        forall (idx: uint256),
-        Primops.memory{1}.[idx] =
-        Primops.memory{2}.[idx]
+lemma usr_pointMulIntoDest_extracted_matches_low (x y : uint256) : equiv [
+    Verifier_1261.usr_pointMulIntoDest ~ PointMulIntoDest.low :
+      ={arg, glob PointMulIntoDest} ==>
+      ={res, glob PointMulIntoDest}
     ].
 proof.
   proc.
-  seq 17 7: (#pre /\ ={_1} /\ _2{1} = W256.zero /\ _3{1} = W256.of_int 32 /\ _4{1} = usr_point{1} + _3{1}
-            /\ _6{1} = W256.of_int 64 /\ _7{1} = W256.of_int 96 /\ _8{1} = W256.of_int 7 /\ ={_5, _9, _10}).
-  inline*. wp. skip. progress.
-  inline*. wp. skip. progress.
+  seq 17 7: (#pre /\ ={_10}).
+  inline*. wp. skip. by progress.
+  inline*. wp. skip. by progress.
 qed.
