src/All.ec
@@ -15,6 +15,11 @@ require EvaluateLagrangePolyOutOfDomain.
 require LookupQuotientContribution.
 require Modexp.
 require PermutationQuotientContribution.
+require PointAddAssign.
+require PointAddIntoDest.
+require PointMulAndAddIntoDest.
+require PointMulIntoDest.
 require PointNegate.
+require PointSubAssign.
 require RevertWithMessage.
 require VerifyQuotientEvaluation.
